work on RLP, sender recovery, state root

Blanc.lean
@@ -1,18 +1,36 @@
+import Lean.Data.Json
+import Lean.Data.Json.Parser
 import «Blanc».Weth
 
-partial def Bytes.chunks (bs : Bytes) : List Bytes :=
-  match bs.splitAt 32 with
-  | (_, []) => [bs]
-  | (bs', bs'') => bs' :: chunks bs''
+
+def List.chunksCore {ξ} (m : Nat) : Nat → List ξ → List (List ξ)
+  | _, [] => [[]]
+  | 0, x :: xs =>
+    match chunksCore m m xs with
+    | [] => [[], [x]]
+    | ys :: yss => [] :: (x :: ys) :: yss
+  | n + 1, x :: xs =>
+    match chunksCore m n xs with
+    | [] => [[x]]
+    | ys :: yss => (x :: ys) :: yss
+
+
+def List.chunks {ξ} (m : Nat) : List ξ → List (List ξ) := List.chunksCore m (m + 1)
+
+-- #exit
+-- partial def Bytes.chunks (bs : Bytes) : List Bytes :=
+--   match bs.splitAt 32 with
+--   | (_, []) => [bs]
+--   | (bs', bs'') => bs' :: chunks bs''
 
 def Bytes.toHexLine (bs : Bytes) : String :=
-  s!"hex\"{bs.toHextring}\""
+  s!"hex\"{bs.toHex}\""
 
 def WethByteCode : String :=
   List.foldr
      (λ s0 s1 => s0 ++ "\n" ++ s1)
      "" <| List.map Bytes.toHexLine
-        <| Bytes.chunks <| Option.getD weth.compile []
+        <| List.chunks 31 <| Option.getD weth.compile []
 
 -- def main : IO Unit := IO.println WethByteCode
 
@@ -43,12 +61,13 @@ def Bytes.toNat' : Nat → Bytes → Nat
 def Bytes.toNat (bs : Bytes) : Nat := bs.toNat' 0
 
 
-def Nat.toBytes' (n : Nat) : Bytes :=
+def Nat.toBytesCore (n : Nat) : Bytes :=
   if n < 256
   then [n.toByte]
-  else (n % 256).toByte :: (n / 256).toBytes'
+  else (n % 256).toByte :: (n / 256).toBytesCore
 
-def Nat.toBytes (n : Nat) : Bytes := n.toBytes'.reverse
+def Nat.toBytes (n : Nat) : Bytes := n.toBytesCore.reverse
+
 
 mutual
   def RLP.decode' : Nat → Bytes → Option (RLP × Bytes)
@@ -120,34 +139,43 @@ mutual
 end
 
 partial def RLP.toStrings : RLP → List String
-  | .bytes bs => [s!"0x{bs.toHextring}"]
+  | .bytes bs => [s!"0x{bs.toHex}"]
   | .list rs => "List:" :: (rs.map RLP.toStrings).flatten.map ("  " ++ ·)
 
 def Strings.join : List String → String
   | [] => ""
   | s :: ss => s ++ "\n" ++ Strings.join ss
 
-def Hexes.toBytes : List Hex → Option Bytes
+def Nibs.toBytes : List Nib → Option Bytes
   | [] => some []
   | [_] => none
-  | h0 :: h1 :: hs => (Ox h0 h1 :: ·) <$> Hexes.toBytes hs
+  | h0 :: h1 :: hs => (Ox h0 h1 :: ·) <$> Nibs.toBytes hs
 
-def Hextring.toBytes (s : String) : Option Bytes :=
-  Hexes.toBytes <| s.data.map Hexar.toHex
+def Hex.toBytes (s : String) : Option Bytes :=
+  s.data.mapM Hexit.toNib >>= Nibs.toBytes
+
+#eval (RLP.encode (.list [])).toHex
 
 def notTxBytes : Bytes :=
-  (Hextring.toBytes "f885800a8404c4b40094cccccccccccccccccccccccccccccccccccccccc01a4693c613900000000000000000000000000000000000000000000000000000000000000001ba0e8ff56322287185f6afd3422a825b47bf5c1a4ccf0dc0389cdc03f7c1c32b7eaa0776b02f9f5773238d3ff36b74a123f409cd6420908d7855bbe4c8ff63e00d698").getD []
+  (Hex.toBytes "f885800a8404c4b40094cccccccccccccccccccccccccccccccccccccccc01a4693c613900000000000000000000000000000000000000000000000000000000000000001ba0e8ff56322287185f6afd3422a825b47bf5c1a4ccf0dc0389cdc03f7c1c32b7eaa0776b02f9f5773238d3ff36b74a123f409cd6420908d7855bbe4c8ff63e00d698").getD []
+
+def badTxBytes : Bytes :=
+  (Hex.toBytes "f885800a8404c4b40094ccccc76482364981768476182936712638712ccc01a4693c613900000000000000000000000000000000000000000000000000000000000000001ba0e8ff56322287185f6afd3422a825b47bf5c1a4ccf0dc0389cdc03f7c1c32b7eaa0776b02f9f5773238d3ff36b74a123f409cd6420908d7855bbe4c8ff63e00d698").getD []
 
 def highValueTxBytes : Bytes :=
-  (Hextring.toBytes "f87f800182520894095e7baea6a6c7c4c2dfeb977efac326af552d87a0ffffffffffffffffffffffffffffffffffffffffffffffffffffffffffffffff801ba048b55bfa915ac795c431978d8a6a992b628d557da5ff759b307d495a36649353a01fffd310ac743f371de3b9f7f9cb56c0b28ad43601b4ab949f53faa07bd2c804").getD []
+  (Hex.toBytes "f87f800182520894095e7baea6a6c7c4c2dfeb977efac326af552d87a0ffffffffffffffffffffffffffffffffffffffffffffffffffffffffffffffff801ba048b55bfa915ac795c431978d8a6a992b628d557da5ff759b307d495a36649353a01fffd310ac743f371de3b9f7f9cb56c0b28ad43601b4ab949f53faa07bd2c804").getD []
 
-def optionToIO {ξ} (o : Option ξ) : IO ξ := do
+def Option.toIO {ξ} (o : Option ξ) (msg : String) : IO ξ := do
   match o with
-  | none => throw (IO.Error.userError "none value")
+  | none => throw (IO.Error.userError msg)
   | some x => pure x
 
-@[extern "ecrecover"]
-opaque ecrecover : ByteArray → ByteArray → ByteArray
+@[extern "ecrecover_flag"]
+opaque ecrecoverFlag : ByteArray → UInt8 → ByteArray → ByteArray
+
+def Bool.toByte : Bool → Byte
+  | true => Ox x0 x1
+  | false => Ox x0 x0
 
 def Byte.toUInt8 (b : Byte) : UInt8 := ⟨⟨b.toNat, b.toNat_lt_pow⟩⟩
 def UInt8.toByte (i : UInt8) : Byte := i.toBitVec.toFin.val.toByte
@@ -155,25 +183,694 @@ def UInt8.toByte (i : UInt8) : Byte := i.toBitVec.toFin.val.toByte
 def Bytes.toBytesArray (bs : Bytes) : ByteArray := ⟨⟨List.map Byte.toUInt8 bs⟩⟩
 def ByteArray.toBytes (a : ByteArray) : Bytes := a.data.toList.map UInt8.toByte
 
+def ecrecover (h : Word) (v : Bool) (r : Word) (s : Word) : Option Addr :=
+  let rsa : ByteArray := Bytes.toBytesArray <| @Bits.toBytes 64 (r ++ s)
+  let hsa : ByteArray := Bytes.toBytesArray (@Bits.toBytes 32 h)
+  let ri : UInt8 := if v then 1 else 0
+  match (ecrecoverFlag hsa ri rsa).toBytes with
+  | [] => none
+  | b :: pa =>
+    if b = 0 ∨ pa.length ≠ 20
+    then none
+    else some (Bytes.toBits 20 pa)
+
+def readJsonFile (filename : System.FilePath) : IO Lean.Json := do
+  let contents ← IO.FS.readFile filename
+  match Lean.Json.parse contents with
+  | .ok json => pure json
+  | .error err => throw (IO.userError err)
+
+-- inductive Json where
+--   | null
+--   | bool (b : Bool)
+--   | num (n : JsonNumber)
+--   | str (s : String)
+--   | arr (elems : Array Json)
+--   -- uses RBNode instead of RBMap because RBMap is a def
+--   -- and thus currently cannot be used to define a type that
+--   -- is recursive in one of its parameters
+--   | obj (kvPairs : RBNode String (fun _ => Json))
+--   deriving Inhabited
+
+
+mutual
+  partial def StringJsons.toStrings : List ((_ : String) × Lean.Json) → List String
+    | [] => []
+    | sj :: sjs =>
+      (sj.fst :: Lean.Json.toStrings sj.snd) ++ StringJsons.toStrings sjs
+
+  partial def Lean.Jsons.toStrings : List Lean.Json → List String
+    | [] => []
+    | j :: js => Lean.Json.toStrings j ++ Lean.Jsons.toStrings js
+
+  partial def Lean.Json.toStrings : Lean.Json → List String
+    | .null => ["null"]
+    | .bool b => [s!"bool : {b}"]
+    | .num n => [s!"num : {n}"]
+    | .str s => [s!"str : {s}"]
+    | .arr js =>
+      "arr :" :: (Lean.Jsons.toStrings js.toList).map ("  " ++ ·)
+    | .obj m => do
+      let kvs := m.toArray.toList
+      "obj : " :: (StringJsons.toStrings kvs).map ("  " ++ ·)
+end
+
+def Lean.Json.toString (j : Lean.Json) : String := Strings.join j.toStrings
+
+def Bits.ordering {n} (xs ys : Bits n) : Ordering :=
+  if xs < ys
+  then .lt
+  else if xs = ys
+       then .eq
+       else .gt
+
+instance {n} : Ord (Bits n) := ⟨Bits.ordering⟩
+
+-- def Stor := Lean.RBMap Word Word Ord.compare
+
+def List.compare {ξ : Type u} [Ord ξ] : List ξ → List ξ → Ordering
+  | [], [] => .eq
+  | [], _ :: _ => .lt
+  | _ :: _, [] => .gt
+  | x :: _, y :: _ => Ord.compare x y
+
+instance {ξ : Type u} [Ord ξ] : Ord (List ξ) := ⟨List.compare⟩
+
+abbrev NTB := Lean.RBMap Nibs Bytes compare
+abbrev Stor := Lean.RBMap Word Word compare
+
+structure PreAcct where
+  (addr : Addr)
+  (nonce : Bytes)
+  (bal : Bytes)
+  (stor : Stor)
+  (code : Bytes)
+
+structure PostAcct where
+  (hash : Word)
+  (dataIdx : Nat)
+  (gasIdx : Nat)
+  (valueIdx : Nat)
+  (logs : Word)
+  (txdata : Bytes)
+
+structure TX : Type where
+  (data : List Bytes)
+  (gasLimit : List Word)
+  (gasPrice : Word)
+  (nonce : Word)
+  (secretKey : Word)
+  (sender : Addr)
+  (receiver : Addr)
+  (value : List Word)
+
+structure TestFile where
+  (info : Lean.Json)
+  (env  : Lean.Json)
+  (pre  : List PreAcct)
+  (post : String × List PostAcct)
+  (tx   : TX)
+
+structure Test where
+  (pre  : List PreAcct)
+  (txdata : Bytes)
+  (data : Bytes)
+  (gasLimit : Word)
+  (gasPrice : Word)
+  (nonce : Word)
+  (secretKey : Word)
+  (sender : Addr)
+  (receiver : Addr)
+  (value : Word)
+  (hash : Word) -- ?
+  (logs : Word) -- keccak hash of (RLP-encoded) log items
+
+def pad : String → String
+  | s => "  " ++ s
+
+def padMid : String -> String
+  | s => "│ " ++ s
+
+def padsMid : List String → List String
+  | [] => []
+  | s :: ss => ("├─" ++ s) :: ss.map padMid
+
+def padsEnd : List String → List String
+  | [] => []
+  | s :: ss => ("└─" ++ s) :: ss.map pad
+
+def padss : List (List String) -> List String
+  | [] => []
+  | [ss] => padsEnd ss
+  | ss :: sss => padsMid ss ++ padss sss
+
+def fork (s : String) : List (List String) → List String
+  | [[s']] => [s ++ "──" ++ s']
+  | sss => s :: padss sss
+
+def encloseStrings : List String → List String
+  | [] => ["[]"]
+  | [s] => ["[" ++ s ++ "]"]
+  | ss => "┌─" :: ss.map padMid ++ ["└─"]
+
+def listToStrings {ξ} (f : ξ -> List String) (xs : List ξ) : List String :=
+  encloseStrings (xs.map f).flatten
+
+def txdataToStrings (tx : Bytes) : List String :=
+  match List.chunks 31 tx with
+  | [] => ["txdata :"]
+  | [bs] => [s!"txdata : {Bytes.toHex bs}"]
+  | bss => "txdata :" :: bss.map (λ bs => pad (Bytes.toHex bs))
+
+def postAcct.toStrings (p : PostAcct) : List String :=
+  fork "Post Acct" [
+    [s!"hash : {Bits.toHex 64 p.hash}"],
+    [s!"data index : {p.dataIdx}"],
+    [s!"gas index : {p.gasIdx}"],
+    [s!"value index : {p.valueIdx}"],
+    [s!"logs : {Bits.toHex 64 p.logs}"],
+    txdataToStrings p.txdata
+  ]
+
+def Stor.toStrings (s : Stor) : List String :=
+  let kvs := s.toArray.toList
+  let kvToStrings : Word × Word → List String :=
+    λ nb => [s!"{nb.fst.toString} : {nb.snd.toString}"]
+  fork "stor" (kvs.map kvToStrings)
+
+#check Bytes.toHex
+
+def NTB.toStrings (s : NTB) : List String :=
+  let kvs := s.toArray.toList
+  let kvToStrings : Nibs × Bytes → List String :=
+    λ nb => [s!"{nb.fst.toHex} : {nb.snd.toHex}"]
+  fork "NTB" (kvs.map kvToStrings)
+
+def preAcct.toStrings (p : PreAcct) : List String :=
+  fork "Pre Acct" [
+    [s!"address : {Bits.toHex 40 p.addr}"],
+    [s!"nonce : {Bytes.toHex p.nonce}"],
+    [s!"balance : {Bytes.toHex p.bal}"],
+    p.stor.toStrings,
+    [s!"code : {Bytes.toHex p.code}"]
+  ]
+
+def postToStrings : (String × List PostAcct) → List String
+  | ⟨s, ps⟩ => fork "Post" [[s], listToStrings postAcct.toStrings ps]
+
+def preToStrings (l : List PreAcct) : List String :=
+  fork "pre" [listToStrings preAcct.toStrings l]
+
+def TX.toStrings (tx : TX) : List String :=
+  fork "transaction" [
+    fork "data" [listToStrings (λ x => [Bytes.toHex x]) tx.data],
+    fork "gasLimit" [listToStrings (λ x => [Bits.toHex 64 x]) tx.gasLimit],
+    [s!"gasPrice : {Bits.toHex 64 tx.gasPrice}"],
+    [s!"nonce : {Bits.toHex 64 tx.nonce}"],
+    [s!"secretKey : {Bits.toHex 64 tx.secretKey}"],
+    [s!"sender : {Bits.toHex 40 tx.sender}"],
+    [s!"to : {Bits.toHex 40 tx.receiver}"],
+    fork "value" [listToStrings (λ x => [Bits.toHex 64 x]) tx.value]
+  ]
+
+def TestFile.toStrings (t : TestFile) : List String :=
+  fork "VM Test" [
+    ["info ..."],--t.info.toStrings,
+    ["env ..."],--t.env.toStrings,
+    preToStrings t.pre,
+    postToStrings t.post,
+    t.tx.toStrings
+  ]
+
+def TestFile.toString (t : TestFile) : String := Strings.join t.toStrings
+
+def IO.throw {ξ} (s : String) : IO ξ := MonadExcept.throw <| IO.Error.userError s
+
+def Lean.Json.fromArr : Lean.Json → IO (List Json)
+  | .arr a => return a.toList
+  | _ => IO.throw "not an array"
+
+def Lean.Json.fromObj : Lean.Json → IO (RBNode String (λ _ => Json))
+  | .obj r => return r
+  | _ => IO.throw "not an object"
+
+def Lean.Json.fromStr : Lean.Json → IO String
+  | .str s => return s
+  | _ => IO.throw "not a string"
+
+def Lean.Json.fromNum : Lean.Json → IO JsonNumber
+  | .num n => return n
+  | _ => IO.throw "not a string"
+
+def Lean.JsonNumber.toString' : JsonNumber → String
+  | ⟨x, y⟩ => s!"<mantissa : {x}, exponent : {y}>"
+
+def Lean.JsonNumber.toNat : JsonNumber → IO Nat
+  | ⟨.ofNat x, 0⟩ => return x
+  | ⟨.negSucc _, _⟩ => IO.throw "negative mantissa"
+  | ⟨_, e + 1⟩ => IO.throw s!"nonzero exponent : {e + 1}"
+
+def Lean.Json.fromSingleton : Lean.Json → IO (String × Lean.Json)
+  | .obj (.node _ .leaf k v .leaf) => return ⟨k, v⟩
+  | _ => IO.throw "not a singleton"
+
+def Hex.from0x : String → IO String
+  | ⟨'0' :: 'x' :: s⟩ => return ⟨s⟩
+  | _ => IO.throw "prefix not 0x"
+
+def Lean.Json.toPostAcct : Json → IO PostAcct
+  | .obj r => do
+    let hsx ← (r.find compare "hash").toIO "cannot retrieve hash bytes" >>= fromStr >>= Hex.from0x
+    let hs ← (Hex.toBits 64 hsx).toIO "cannot convert hash bytes to word"
+    let lgx ← (r.find compare "logs").toIO "cannot get logs bytes" >>= fromStr >>= Hex.from0x
+    let lg ← (Hex.toBits 64 lgx).toIO "cannot convert logs bytes to word"
+    let txx ← (r.find compare "txbytes").toIO "cannot get tx bytes" >>= fromStr >>= Hex.from0x
+    let tx ← (Hex.toBytes txx).toIO "cannot convert tx bytes to word"
+    let dgv ← (r.find compare "indexes").toIO "cannot get indexes" >>= Json.fromObj
+    let d ← (dgv.find compare "data").toIO "cannot get data" >>= Json.fromNum >>= JsonNumber.toNat
+    let g ← (dgv.find compare "gas").toIO "cannot get gas" >>= Json.fromNum >>= JsonNumber.toNat
+    let v ← (dgv.find compare "value").toIO "cannot get value" >>= Json.fromNum >>= JsonNumber.toNat
+    return ⟨hs, d, g, v, lg, tx⟩
+  | _ => IO.throw "Json-to-PostAcct failed"
+
+
+-- def kbAdd {ξ υ o} (s : Lean.RBMap ξ υ o) (kv : (_ : String) × Json) : IO Stor := return s
+
+def Lean.Json.toBytes (j : Json) : IO Bytes := do
+  let x ← fromStr j >>= Hex.from0x
+  (Hex.toBytes x).toIO ""
+
+def Lean.Json.toBits (n : Nat) (j : Json) : IO (Bits (4 * n)) := do
+  let x ← fromStr j >>= Hex.from0x
+  (Hex.toBits n x).toIO ""
+
+
+def Lean.Json.toPreAcct (sj : (_ : String) × Json) : IO PreAcct := do
+  -- let a ← Hex.from0x sj.fst >>= (Option.toIO ∘ Hex.toBits 40)
+  let ax ← Hex.from0x sj.fst
+  let a ← (Hex.toBits 40 ax).toIO ""
+  let r ← sj.snd.fromObj
+  let b ← ((r.find Ord.compare "balance").toIO "" >>= toBytes) --<&> Bytes.toBits 32
+  let c ← (r.find Ord.compare "code").toIO "" >>= toBytes
+  let n ← ((r.find Ord.compare "nonce").toIO "" >>= toBytes) -- <&> Bytes.toBits 32
+  --let sr ← (r.find Ord.compare "storage").toIO >>= fromObj
+  --let kvs := sr.toArray.toList
+  --let s ← kvs.foldlM Stor.add (Lean.RBMap.empty : Stor)
+  return ⟨a, n, b, Lean.RBMap.empty, c⟩
+
+def Lean.Json.toPre (j : Lean.Json) : IO (List PreAcct) := do
+  let r ← j.fromObj
+  let kvs := r.toArray.toList
+  mapM Lean.Json.toPreAcct kvs
+
+def Lean.Json.toPost (j : Lean.Json) : IO (String × List PostAcct) := do
+  let ⟨k, j'⟩ ← j.fromSingleton
+  let l ← j'.fromArr
+  let js ← mapM Lean.Json.toPostAcct l
+  return ⟨k, js⟩
+
+def Bytes.toWord : Bytes → Word := Bytes.toBits 32
+
+def Lean.Json.toTX (j : Lean.Json) : IO TX := do
+  let r ← j.fromObj
+  let ds ← (r.find Ord.compare "data").toIO "" >>= fromArr >>= mapM toBytes
+  let gls ← (r.find Ord.compare "gasLimit").toIO "" >>= fromArr >>= mapM toBytes
+  let gp ← ((r.find Ord.compare "gasPrice").toIO "" >>= toBytes) <&> Bytes.toWord
+  let n ← ((r.find Ord.compare "nonce").toIO "" >>= toBytes) <&> Bytes.toWord
+  let sk ← (r.find Ord.compare "secretKey").toIO "" >>= toBits 64
+  let sd ← (r.find Ord.compare "sender").toIO "" >>= toBits 40
+  let rc ← (r.find Ord.compare "to").toIO "" >>= toBits 40
+  let vs ← (r.find Ord.compare "value").toIO "" >>= fromArr >>= mapM toBytes
+  return ⟨ds, gls.map Bytes.toWord, gp, n, sk, sd, rc, vs.map Bytes.toWord⟩
+
+def Lean.Json.toTestFile (j : Lean.Json) : IO TestFile := do
+  let (_, .obj r) ← j.fromSingleton | IO.throw "not singleton object"
+  let info ← (r.find compare "_info").toIO ""
+  let env ←  (r.find compare "env").toIO ""
+  let pre ←  (r.find compare "pre").toIO "" >>= Lean.Json.toPre
+  let post ← (r.find compare "post").toIO "" >>= Lean.Json.toPost
+  let tx ←   (r.find compare "transaction").toIO "" >>= Lean.Json.toTX
+  return ⟨info, env, pre, post, tx⟩
+
+-- structure PostAcct where
+--   (hash : Word)
+--   (dataIdx : Nat)
+--   (gasIdx : Nat)
+--   (valueIdx : Nat)
+--   (logs : Word)
+--   (txdata : Bytes)
+--
+-- structure TX : Type where
+--   (data : List Bytes)
+--   (gasLimit : List Word)
+--   (gasPrice : Word)
+--   (nonce : Word)
+--   (secretKey : Word)
+--   (sender : Addr)
+--   (receiver : Addr)
+--   (value : List Word)
+
+def getTest (ps : List PreAcct) (tx : TX) (p : PostAcct) : IO Test := do
+  let d ← (List.get? tx.data p.dataIdx).toIO ""
+  let gl ← (List.get? tx.gasLimit p.gasIdx).toIO ""
+  let vl ← (List.get? tx.value p.valueIdx).toIO ""
+  return {
+    pre := ps
+    txdata := p.txdata
+    data := d
+    gasLimit := gl
+    gasPrice := tx.gasPrice
+    nonce := tx.nonce
+    secretKey := tx.secretKey
+    sender := tx.sender
+    receiver := tx.receiver
+    value := vl
+    hash := p.hash
+    logs := p.logs
+  }
+
+def getTests (t : TestFile) : IO (List Test) := do
+  have ps := t.post.snd
+  mapM (getTest t.pre t.tx) ps
+
+def Lean.RBMap.fromSingleton {ξ υ f} (m : RBMap ξ υ f) : Option (ξ × υ) :=
+  match m.toList with
+  | [kv] => some kv
+  | _ => none
+
+def Lean.RBMap.singleton {ξ υ f} (x : ξ) (y : υ) : RBMap ξ υ f := RBMap.empty.insert x y
+
+def hpAux : Nibs → (Option Nib × Bytes)
+  | [] => ⟨none, []⟩
+  | n :: ns =>
+    match hpAux ns with
+    | ⟨none, bs⟩ => ⟨some n, bs⟩
+    | ⟨some m, bs⟩ => ⟨none, (n ++ m) :: bs⟩
+
+def hp (ns : Nibs) (t : Bool) : Bytes :=
+  match hpAux ns with
+  | ⟨none, bs⟩ => ⦃0, 0, t, 0, 0, 0, 0, 0⦄ :: bs
+  | ⟨some n, bs⟩ => (⦃0, 0, t, 1⦄ ++ n) :: bs
+
+
+def commonPrefixCore : Nibs → Nibs → Nibs
+  | [], _ => []
+  | _, [] => []
+  | n :: ns, n' :: ns' =>
+    if n = n' then n :: commonPrefixCore ns ns'
+    else []
+
+def commonPrefix (n : Nib) (ns : Nibs) : List Nibs → Option Nibs
+  | [] => some (n :: ns)
+  | ns' :: nss =>
+    match commonPrefixCore (n :: ns) ns' with
+    | [] => none
+    | (n' :: ns'') => commonPrefix n' ns'' nss
+
+
+def NTB.empty : NTB := Lean.RBMap.empty
+
+def sansPrefix : Nibs → Nibs → Option Nibs
+  | [], ns => some ns
+  | _, [] => none
+  | n :: ns, n' :: ns' =>
+    if n = n' then sansPrefix ns ns' else none
+
+def insertSansPrefix (pfx : Nibs) (m : NTB) (ns : Nibs) (bs : Bytes) : Option NTB := do
+  (m.insert · bs) <$> sansPrefix pfx ns
+
+def NTB.factor (m : NTB) : Option (Nibs × NTB) := do
+  let ((n :: ns) :: nss) ← some (m.toList.map Prod.fst) | none
+  let pfx ← commonPrefix n ns nss
+  let m' ← Lean.RBMap.foldM (insertSansPrefix pfx) NTB.empty m
+  some ⟨pfx, m'⟩
+
+structure NTBs : Type where
+  (x0 : NTB) (x1 : NTB) (x2 : NTB) (x3 : NTB)
+  (x4 : NTB) (x5 : NTB) (x6 : NTB) (x7 : NTB)
+  (x8 : NTB) (x9 : NTB) (xA : NTB) (xB : NTB)
+  (xC : NTB) (xD : NTB) (xE : NTB) (xF : NTB)
+
+def NTBs.empty : NTBs :=
+  ⟨ .empty, .empty, .empty, .empty,
+    .empty, .empty, .empty, .empty,
+    .empty, .empty, .empty, .empty,
+    .empty, .empty, .empty, .empty ⟩
+
+def NTBs.update (js : NTBs) (f : NTB → NTB) : Nib → NTBs
+  | ⦃0, 0, 0, 0⦄ => { js with x0 := f js.x0}
+  | ⦃0, 0, 0, 1⦄ => { js with x1 := f js.x1}
+  | ⦃0, 0, 1, 0⦄ => { js with x2 := f js.x2}
+  | ⦃0, 0, 1, 1⦄ => { js with x3 := f js.x3}
+  | ⦃0, 1, 0, 0⦄ => { js with x4 := f js.x4}
+  | ⦃0, 1, 0, 1⦄ => { js with x5 := f js.x5}
+  | ⦃0, 1, 1, 0⦄ => { js with x6 := f js.x6}
+  | ⦃0, 1, 1, 1⦄ => { js with x7 := f js.x7}
+  | ⦃1, 0, 0, 0⦄ => { js with x8 := f js.x8}
+  | ⦃1, 0, 0, 1⦄ => { js with x9 := f js.x9}
+  | ⦃1, 0, 1, 0⦄ => { js with xA := f js.xA}
+  | ⦃1, 0, 1, 1⦄ => { js with xB := f js.xB}
+  | ⦃1, 1, 0, 0⦄ => { js with xC := f js.xC}
+  | ⦃1, 1, 0, 1⦄ => { js with xD := f js.xD}
+  | ⦃1, 1, 1, 0⦄ => { js with xE := f js.xE}
+  | ⦃1, 1, 1, 1⦄ => { js with xF := f js.xF}
+
+def NTBs.insert (js : NTBs) : Nibs → Bytes → NTBs
+  | [], _ => js
+  | n :: ns, bs => js.update (Lean.RBMap.insert · ns bs) n
+
+mutual
+  def nodeComp : Nat → NTB → RLP
+    | 0, _ => .bytes []
+    | k + 1, j =>
+      if j.isEmpty
+      then .bytes []
+      else let r := structComp k j
+           if r.encode.length < 32
+           then r
+           else .bytes <| @Bits.toBytes 32 r.encode.keccak
+
+  def structComp : Nat → NTB → RLP
+    | 0, _ => .bytes []
+    | k + 1, j =>
+      if j.isEmpty
+      -- then .list (.replicate 17 <| .bytes []) -- what should be returned
+      then .bytes [] -- what devtools actually return
+      else if j.isSingleton
+           then match j.toList with
+                | [(k, v)] => .list [.bytes (hp k 1), .bytes v]
+                | _ => .bytes [] -- unreachable code
+           else match j.factor with
+                | none =>
+                  let js := Lean.RBMap.fold NTBs.insert NTBs.empty j
+                  .list [ nodeComp k js.x0, nodeComp k js.x1, nodeComp k js.x2,
+                          nodeComp k js.x3, nodeComp k js.x4, nodeComp k js.x5,
+                          nodeComp k js.x6, nodeComp k js.x7, nodeComp k js.x8,
+                          nodeComp k js.x9, nodeComp k js.xA, nodeComp k js.xB,
+                          nodeComp k js.xC, nodeComp k js.xD, nodeComp k js.xE,
+                          nodeComp k js.xF, .bytes (j.findD [] []) ]
+                | some (pfx, j') => .list [.bytes (hp pfx 0), nodeComp k j']
+end
+
+
+def List.maxD {ξ} [Max ξ] : List ξ → ξ → ξ
+  | [], y => y
+  | x :: xs, y => maxD xs (max x y)
+
+def NTB.maxKeyLength (j : NTB) : Nat := (j.toList.map (List.length ∘ Prod.fst)).maxD 0
+
+def collapse (j : NTB) : RLP := structComp (2 * (j.maxKeyLength + 1)) j
+
+def trie (j : NTB) : Word := (collapse j).encode.keccak
+
+def Word.toBytes (w : Word) : Bytes :=
+  (@Bits.toBytes 32 w)
+
+def Word.toRLP (w : Word) : RLP := .bytes w.toBytes
+
+def Word.keccak (w : Word) : Word := (@Bits.toBytes 32 w).keccak
+
+def Stor.toNTB (s : Stor) : NTB :=
+  let f : NTB → Word → Word → NTB :=
+    λ j k v =>
+      j.insert
+        (@Bits.toNibs 64 k.keccak)
+        (RLP.encode <| .bytes <| @Bits.toBytes 32 v)
+  Lean.RBMap.fold f NTB.empty s
+
+def PreAcct.toKV (a : PreAcct) : Nibs × Bytes :=
+  ⟨
+    @Bits.toNibs 64 (@Bits.toBytes 20 a.addr).keccak,
+    RLP.encode <| .list [
+      .bytes a.nonce,
+      .bytes a.bal,
+      Word.toRLP (trie a.stor.toNTB),
+      Word.toRLP <| Bytes.keccak a.code
+    ]
+  ⟩
+
+def testStor : Stor :=
+  Lean.RBMap.singleton 0
+    ((Hex.toWord "fffffffffffffffffffffffffffffffffffffffffffffffffedcba9876543210").getD 0)
+
+def testPreAcct1 : PreAcct :=
+  {
+    addr := (Hex.toBits 40 "0000000000000000000000000000000000001000").getD 0
+    nonce := []
+    bal := (Hex.toBytes "0ba1a9ce0ba1a9ce").getD []
+    stor := testStor
+    code := (Hex.toBytes "670123456789abcdef1960005500").getD []
+  }
+
+def testPreAcct2 : PreAcct :=
+  {
+    addr := (Hex.toBits 40 "a94f5374fce5edbc8e2a8697c15331677e6ebf0b").getD 0
+    nonce := [Ox x0 x1]
+    bal := (Hex.toBytes "0ba1a9ce0b9aa79f").getD []
+    stor := .empty
+    code := []
+  }
+
+def testPreAcct3 : PreAcct :=
+  {
+    addr := (Hex.toBits 40 "cccccccccccccccccccccccccccccccccccccccc").getD 0
+    nonce := []
+    bal := (Hex.toBytes "0ba1a9ce0ba1a9cf").getD []
+    stor := .empty
+    code := (Hex.toBytes "600060006000600060006004356110000162fffffff100").getD []
+  }
+
+def testPreAccts : List PreAcct := [testPreAcct1, testPreAcct2, testPreAcct3]
+
+def testNTB : NTB := Lean.RBMap.fromList (List.map PreAcct.toKV testPreAccts) compare
+
+-- def main : IO Unit := do IO.println <| Bits.toHex 64 (trie testNTB)
+
+-- def main : IO Unit := do
+--   let t ← readJsonFile "not.json" >>= Lean.Json.toTestFile
+--   IO.println t.toString
+
+def callData : Bytes :=
+  (Hex.toBytes "693c6139").getD []
+
+def dataGas (cd : Bytes) : Nat :=
+  let aux : Byte → Nat := fun b => if b = 0 then 4 else 16
+  (cd.map aux).sum
+
+def G_initcodeword : Nat := 2
+
+def initCodeCost (cd : Bytes) : Nat :=
+  G_initcodeword * ((cd.length / 32) + if 32 ∣ cd.length then 0 else 1)
+
+def G_txcreate : Nat := 32000
+def G_accesslistaddress : Nat := 2400
+def G_accessliststorage : Nat := 1900
+
+def intrinsicGas (Tt : Bytes) (cd : Bytes) (Ta : List (Addr × List Word)) : Nat :=
+  let aux : (Addr × List Word) → Nat :=
+    fun | ⟨_, l⟩ => G_accesslistaddress + (G_accessliststorage * l.length)
+  dataGas cd +
+  (if Tt = [] then G_txcreate + initCodeCost cd else 0) +
+  2100 +
+  (Ta.map aux).sum
+
+def Tg : Nat := ((Hex.toBytes "04C4B400").getD []).toNat
+
+def g : Nat := Tg - intrinsicGas ((Hex.toBytes "cccccccccccccccccccccccccccccccccccccccc").getD []) callData []
+
+def C : Nat := _ + _
+
+def g' : Nat := g - C
+
+structure Acct where
+  (nonce : Word)
+  (bal : Word)
+  (stor : Stor)
+  (code : Bytes)
+
+abbrev World' : Type := Lean.RBMap Addr Acct compare
+
+structure State' where
+  (w : World')
+  (cta : Addr)
+  (pc : Nat)
+
+def testWorld : World' :=
+  let aux : PreAcct → (Addr × Acct) :=
+    fun pa => ⟨pa.addr, ⟨pa.nonce.toBits 32, pa.bal.toBits 32, pa.stor, pa.code⟩⟩
+  Lean.RBMap.fromList (testPreAccts.map aux) _
+
+def testState : State' :=
+  {
+    w := testWorld
+    cta := (Hex.toBits 40 "cccccccccccccccccccccccccccccccccccccccc").getD 0
+    pc := 0
+  }
+
+def State'.inst (s : State') : IO (Inst ⊕ Hinst) := do
+  let a ← (s.w.find? s.cta).toIO "contract does not exist in state"
+  match a.code.get? s.pc with
+  | none =>
+    if a.code.length = s.pc
+    then return (.inr .stop)
+    else .throw "unreachable code : out-of-bound instruction lookup inconsistent with normal usage"
+  | some b => _
+
+#exit
+
+def State'.gas (s : State') : IO Nat := do
+  let a ← (s.w.find? s.cta).toIO "cannot get acct"
+  let c ← (a.code.get? s.pc).toIO "cannot"
+
+  _
+
+
+#exit
+
+
+def Bits.min {n} : Bits n → Bits n → Bits n
+  | xs, ys => if xs ≤ ys then xs else ys
+
+instance {n} : Min (Bits n) := ⟨.min⟩
+
+def A_r : Word := 0 -- SSTORE used only once, cannot change from 0
+
+def gstar : Word := g' + min ((Tg - gprime) / 5) A_r
+
+def balInit : Word := Bytes.toWord ((Hex.toBytes "0ba1a9ce0ba1a9ce").getD [])
+
+def txVal : Word := 1
+
+def Yg : Word := Tg - gstar
+
+def gasPrice : Word := 10--Bytes.toWord ((Hex.toBytes "0a").getD [])
+
+def balFinal : Word := balInit - ((Yg * gasPrice) + txVal)
+
+
+#exit
+
+
 def main : IO Unit := do
-  let bs := highValueTxBytes
-  let (RLP.list [txType, nonce, gasPrice, toAddr, val, calldata, .bytes v, .bytes r, .bytes s])
-    ← (optionToIO <| RLP.decode bs)
-    | throw (IO.Error.userError "Error : decoded list length ≠ 9")
+  let bs := notTxBytes
+  let (RLP.list [nonce, gasPrice, gasLimit, toAddr, val, calldata, .bytes [v], .bytes r, .bytes s])
+    ← (Option.toIO <| RLP.decode bs)
+    | throw (IO.Error.userError "Error : RLP decoding failed")
   let bs' := RLP.encode <| .list [txType, nonce, gasPrice, toAddr, val, calldata]
   let hs := bs'.keccak
 
-  IO.println <| s!"v : {v.toNat}"
-  IO.println <| s!"r : {r.toHextring}"
-  IO.println <| s!"s : {s.toHextring}"
-  IO.println <| s!"Hash of txdata excluding signature: {Bits.toHextring 32 hs}"
+  IO.println <| s!"v : {Bits.toHex 2 v}"
+  IO.println <| s!"r : {r.toHex}"
+  IO.println <| s!"s : {s.toHex}"
+  IO.println <| s!"Hash of txdata excluding signature: {Bits.toHex 64 hs}"
 
   let rsa : ByteArray := Bytes.toBytesArray (r ++ s)
   let hsa : ByteArray := Bytes.toBytesArray (@Bits.toBytes 32 hs)
+  let ri : UInt8 := Byte.toUInt8 (v - Ox x1 xB)
 
-  match (ecrecover rsa hsa).toBytes with
+  match (ecrecoverFlag hsa ri rsa).toBytes with
   | [] => IO.println "Unreachable code : ecrecover should never return empty bytes"
   | b :: pa =>
     if b = 0
     then IO.println "ecrecover failed"
-    else IO.println <| s!"Recovered public address : {Bytes.toHextring pa}"
+    else IO.println <| s!"Recovered public address : {Bytes.toHex pa}"
